done/Iron/Language/SystemF2Effect/Step/FreshF.v
@@ -1,0 +1,31 @@
+
+Require Export Iron.Language.SystemF2Effect.Step.Frame.
+
+
+Fixpoint freshF (p : nat) (ff : frame) {struct ff} : Prop := 
+ match ff with
+ | FLet  t x     => freshT p t /\ freshX p x
+ | FPriv p1      => beq_nat p p1 = false
+ | FExt  p1 p2   => beq_nat p p1 = false /\ beq_nat p p2 = false
+ end.
+
+
+Definition freshFs (p : nat) (fs : stack) : Prop
+ := Forall (freshF p) fs.
+Hint Unfold freshFs.
+
+
+Lemma freshFs_head 
+ :  forall p f fs
+ ,  freshFs p (fs :> f)
+ -> freshFs p fs.
+Proof. intros. inverts H. eauto. Qed.
+Hint Resolve freshFs_head.
+
+
+Lemma freshFs_tail
+ :  forall p f fs
+ ,  freshFs p (fs :> f)
+ -> freshF  p f.
+Proof. intros. inverts H. eauto. Qed.
+Hint Resolve freshFs_tail.
