done/Iron/Language/SystemF2Effect/Type/Operator.v
@@ -6,3 +6,4 @@ Require Export Iron.Language.SystemF2Effect.Type.Operator.FlattenT.
 Require Export Iron.Language.SystemF2Effect.Type.Operator.BunchT.
 Require Export Iron.Language.SystemF2Effect.Type.Operator.MaskOnT.
 Require Export Iron.Language.SystemF2Effect.Type.Operator.MaskOnTs.
+Require Export Iron.Language.SystemF2Effect.Type.Operator.MergeT.
