done/Iron/Language/SystemF2Effect/Type/Operator/MergeT.v
@@ -1,0 +1,45 @@
+
+Require Export Iron.Language.SystemF2Effect.Type.Exp.Base.
+Require Export Iron.Language.SystemF2Effect.Type.Operator.SubstTT.
+Require Export Iron.Language.SystemF2Effect.Type.Relation.FreshT.
+
+
+Fixpoint mergeT (p1 p2 : nat) (tt : ty)  : ty :=
+ match tt with
+ | TVar    _            => tt
+ | TForall k t          => TForall k (mergeT p1 p2 t)
+ | TApp    t1 t2        => TApp (mergeT p1 p2 t1) (mergeT p1 p2 t2)
+ | TSum    t1 t2        => TSum (mergeT p1 p2 t1) (mergeT p1 p2 t2)
+ | TBot    k            => TBot k
+ | TCon0   tc0          => TCon0 tc0
+ | TCon1   tc1 t1       => TCon1 tc1 (mergeT p1 p2 t1)
+ | TCon2   tc2 t1 t2    => TCon2 tc2 (mergeT p1 p2 t1) (mergeT p1 p2 t2)
+ | TCap (TyCapRegion p) => if beq_nat p p2 then TRgn p1 else tt
+ end.
+
+
+Lemma mergeT_freshT_id
+ :  forall p1 p2 t
+ ,  freshT p2 t
+ -> mergeT p1 p2 t = t.
+Proof.
+ intros. 
+ induction t; snorm; rewritess; auto.
+ - destruct t. snorm. nope.
+Qed.
+
+
+Lemma mergeT_substTT
+ :  forall ke sp t k p1 p2 ix
+ ,  freshT p2 t
+ -> KindT ke sp t k
+ -> mergeT p1 p2 (substTT ix (TRgn p2) t)
+ =  substTT ix (TRgn p1) t.
+Proof.
+ intros. gen ix ke k.
+ induction t; snorm;
+  try (inverts H0; espread; eauto).
+ - nope.
+Qed.
+
+
