done/Iron/Language/SystemF2Effect/Type/Relation/FreshT.v
@@ -1,0 +1,17 @@
+
+Require Export Iron.Language.SystemF2Effect.Type.Exp.
+
+
+(* Region identifier is fresh with respect to a type. *)
+Fixpoint freshT (p : nat) (tt : ty) : Prop :=
+ match tt with
+ | TVar _         => True
+ | TForall k t    => freshT p t
+ | TApp t1 t2     => freshT p t1 /\ freshT p t2
+ | TSum t1 t2     => freshT p t1 /\ freshT p t2
+ | TBot _         => True
+ | TCon0 _        => True
+ | TCon1 tc t1    => freshT p t1
+ | TCon2 tc t1 t2 => freshT p t1 /\ freshT p t2
+ | TCap  (TyCapRegion n) => beq_nat n p = false
+ end.
