done/Iron/Language/SystemF2Effect/Value.v
@@ -1,14 +1,16 @@
 
 Require Export Iron.Language.SystemF2Effect.Value.Exp.
-Require Export Iron.Language.SystemF2Effect.Value.Lift.
-Require Export Iron.Language.SystemF2Effect.Value.Wf.
-Require Export Iron.Language.SystemF2Effect.Value.SubstTX.
-Require Export Iron.Language.SystemF2Effect.Value.SubstVX.
-Require Export Iron.Language.SystemF2Effect.Value.Merge.
-Require Export Iron.Language.SystemF2Effect.Value.TyJudge.
-Require Export Iron.Language.SystemF2Effect.Value.TyJudge.Unique.
-Require Export Iron.Language.SystemF2Effect.Value.TyJudge.WeakKiEnv.
-Require Export Iron.Language.SystemF2Effect.Value.TyJudge.WeakTyEnv.
-Require Export Iron.Language.SystemF2Effect.Value.TyJudge.WeakStEnv.
-Require Export Iron.Language.SystemF2Effect.Value.TyJudge.WeakStProps.
+Require Export Iron.Language.SystemF2Effect.Value.Operator.LiftX.
+Require Export Iron.Language.SystemF2Effect.Value.Operator.SubstTX.
+Require Export Iron.Language.SystemF2Effect.Value.Operator.SubstVX.
+Require Export Iron.Language.SystemF2Effect.Value.Operator.MergeX.
+Require Export Iron.Language.SystemF2Effect.Value.Relation.Wf.
+Require Export Iron.Language.SystemF2Effect.Value.Relation.FreeXX.
+Require Export Iron.Language.SystemF2Effect.Value.Relation.FreshX.
+Require Export Iron.Language.SystemF2Effect.Value.Relation.TyJudge.
+Require Export Iron.Language.SystemF2Effect.Value.Relation.TyJudge.Unique.
+Require Export Iron.Language.SystemF2Effect.Value.Relation.TyJudge.WeakKiEnv.
+Require Export Iron.Language.SystemF2Effect.Value.Relation.TyJudge.WeakTyEnv.
+Require Export Iron.Language.SystemF2Effect.Value.Relation.TyJudge.WeakStEnv.
+Require Export Iron.Language.SystemF2Effect.Value.Relation.TyJudge.WeakStProps.
 
