done/Iron/Language/SystemF2Effect/Value/Operator/SubstTX.v
@@ -1,8 +1,8 @@
 
 Require Export Iron.Language.SystemF2Effect.Type.
 Require Export Iron.Language.SystemF2Effect.Value.Exp.
-Require Export Iron.Language.SystemF2Effect.Value.Lift.
-Require Export Iron.Language.SystemF2Effect.Value.TyJudge.
+Require Export Iron.Language.SystemF2Effect.Value.Operator.LiftX.
+Require Export Iron.Language.SystemF2Effect.Value.Relation.TyJudge.
 
 
 (********************************************************************)
