done/Iron/Language/SystemF2Effect/Value/Relation/FreeXX.v
@@ -1,0 +1,26 @@
+
+Require Export Iron.Language.SystemF2Effect.Value.Exp.
+
+
+Fixpoint freeXV (n : nat) (vv : val) : Prop :=
+ match vv with
+ | VVar n'            => beq_nat n n' = true
+ | VLoc _             => False
+ | VLam t x           => freeXX (S n) x
+ | VLAM k x           => freeXX n x
+ | VConst _           => False
+ end
+ with   freeXX (n : nat) (xx : exp) : Prop :=
+ match xx with
+ | XVal     v         => freeXV n v
+ | XLet     t x1 x2   => freeXX n x1 \/ freeXX (S n) x2
+ | XApp     v1 v2     => freeXV n v1 \/ freeXV n v2
+ | XAPP     v1  t2    => freeXV n v1
+ | XOp1     op v      => freeXV n v
+ | XPrivate x         => freeXX n x
+ | XExtend  t x       => freeXX n x
+ | XAlloc   t v1      => freeXV n v1
+ | XRead    t v1      => freeXV n v1
+ | XWrite   t v1 v2   => freeXV n v1 \/ freeXV n v2
+ end.
+
