done/Iron/Language/SystemF2Effect/Value/Relation/FreshX.v
@@ -1,0 +1,27 @@
+
+Require Export Iron.Language.SystemF2Effect.Type.
+Require Export Iron.Language.SystemF2Effect.Value.Exp.
+
+
+Fixpoint freshV (p : nat) (vv : val) : Prop :=
+ match vv with 
+ | VVar     _       => True
+ | VLoc     _       => True
+ | VLam     t x     => freshT p t  /\ freshX p x
+ | VLAM     k x     => freshX p x
+ | VConst   _       => True
+ end
+ with    freshX (p : nat) (xx : exp) : Prop :=
+ match xx with
+ | XVal     v       => freshV p v
+ | XLet     t x1 x2 => freshT p t  /\ freshX p x1 /\ freshX p x2
+ | XApp     v1 v2   => freshV p v1 /\ freshV p v2
+ | XAPP     v1 t2   => freshV p v1 /\ freshT p t2
+ | XOp1     op v    => freshV p v
+ | XPrivate x       => freshX p x
+ | XExtend  t x     => freshT p t  /\ freshX p x
+ | XAlloc   t v     => freshT p t  /\ freshV p v
+ | XRead    t v     => freshT p t  /\ freshV p v
+ | XWrite   t v1 v2 => freshT p t  /\ freshV p v1 /\ freshV p v2
+ end.
+
