done/Iron/Language/SystemF2Effect/Value/Relation/TyJudge/WeakKiEnv.v
@@ -1,6 +1,6 @@
 
 Require Import Iron.Language.SystemF2Effect.Type.
-Require Import Iron.Language.SystemF2Effect.Value.TyJudge.
+Require Import Iron.Language.SystemF2Effect.Value.Relation.TyJudge.
 
 
 (* Weakening Kind Env in Type Judgement. *)
